PartialOrderTactic/testing.lean
@@ -1,5 +1,8 @@
 -- import Mathlib.Tactic.Partiarith
 import PartialOrderTactic.Partiarith
+import Lean.Expr
 
-example (a b c : α) [PartialOrder α] (hab : a ≤ b) (hbc : b ≤ c) : a ≤ c :=
-by partiarith
+lemma first (a b c: α) [PartialOrder α] (hab : a ≤ b) (hbc : c = b) : a ≤ c := by partiarith
+
+
+example (a b c d e: α) [PartialOrder α] (hab : a ≤ b) (hac : a ≤ c) (hcb : c ≤ b) (hbd : b ≤ d) (hce : c ≤ e) : a ≤ e := by partiarith
